hoare triples

two_state_model/assert.v
@@ -20,16 +20,18 @@ Module Assert.
   | a_and : asrt -> asrt -> asrt
   | a_or : asrt -> asrt -> asrt
   | a_neg : asrt -> asrt
-  | a_arr : asrt -> asrt -> asrt
   | a_all : var -> asrt -> asrt
   | a_ex : var -> asrt -> asrt
+
+  | a_intl : exp -> asrt
+  | a_extl : exp -> asrt
 
   | a_prt : exp -> asrt
   | a_prt_frm : exp -> exp -> asrt.
 
   Notation "A1 '∧' A2" := (a_and A1 A2)(at level 39).
   Notation "A1 '∨' A2" := (a_or A1 A2)(at level 39).
-  Notation "A1 '⟶' A2" := (a_arr A1 A2)(at level 39).
+(*)  Notation "A1 '⟶' A2" := (a_arr A1 A2)(at level 39).*)
   Notation "'¬' A" := (a_neg A)(at level 39).
 
   Inductive path :=
@@ -84,6 +86,51 @@ Module Assert.
   Definition protected_from (M : module)(σ : config)(α_orig α : addr) :=
     forall p, interpret_αp p σ α_orig = Some (v_addr α) -> is_protected_path M σ α_orig p.
 
+  Class Subst (A B C : Type) : Type :=
+    {
+      sbst : A -> B -> C -> A
+    }.
+
+  Notation "'[' c '/s' b ']' a" := (sbst a b c)(at level 80).
+
+  #[global] Instance exp_subst : Subst exp nat addr:=
+    {
+    sbst :=
+      fix sbst' e n α :=
+          match e with
+          | e_hole m  => if beq_nat n m
+                        then e_val (v_addr α)
+                        else e_hole m
+          | e_fld e' f => e_fld (sbst' e' n α) f
+          | e_class e' C => e_class (sbst' e' n α) C
+          | e_ghost e0 g e1 => e_ghost (sbst' e0 n α) g (sbst' e1 n α)
+          | e_if e0 e1 e2 => e_if (sbst' e0 n α) (sbst' e1 n α) (sbst' e2 n α)
+          | _ => e
+          end
+    }.
+
+  #[global] Instance asrtSubst : Subst asrt nat addr:=
+    {
+    sbst :=
+      fix sbst' A n α :=
+        match A with
+        | a_exp e     => a_exp ([ α /s n ] e)
+        | A1 ∧ A2     => (sbst' A1 n α) ∧ (sbst' A2 n α)
+        | A1 ∨ A2     => (sbst' A1 n α) ∨ (sbst' A2 n α)
+        | ¬ A         => ¬ (sbst' A n α)
+(*)        | A1 ⟶ A2   => (sbst' A1 n α) ⟶ (sbst' A2 n α)*)
+
+        | a_all x A    => a_all x (sbst' A (S n) α)
+        | a_ex x A   => a_ex x (sbst' A (S n) α)
+
+        | a_intl e => a_intl ([α /s n] e)
+        | a_extl e => a_extl ([α /s n] e)
+
+        | a_prt_frm e1 e2 => a_prt_frm ([α /s n] e1) ([α /s n] e2)
+        | a_prt e => a_prt ([α /s n] e)
+        end
+    }.
+
   Inductive sat : module -> config -> asrt -> Prop :=
   | sat_exp : forall M σ e, eval M σ e v_true ->
                        sat M σ (a_exp e)
@@ -98,21 +145,24 @@ Module Assert.
   | sat_or2 : forall M σ A1 A2, sat M σ A2 ->
                            sat M σ (A1 ∨ A2)
 
-  | sat_arr1 : forall M σ A1 A2, nsat M σ A1 ->
-                            sat M σ (A1 ⟶ A2)
-
-  | sat_arr2 : forall M σ A1 A2, sat M σ A2 ->
-                            sat M σ (A1 ⟶ A2)
-
   | sat_neg : forall M σ A, nsat M σ A ->
                        sat M σ (¬ A)
 
   | sat_all : forall M σ x A, (forall α, glob_relevant α σ ->
-                               sat M σ A) ->
+                               sat M σ ([α /s 0] A)) ->
                          sat M σ (a_all x A)
 
   | sat_ex : forall M σ x α A, glob_relevant α σ ->
+                          sat M σ ([α /s 0] A) ->
                           sat M σ (a_ex x A)
+
+  | sat_intl : forall M σ e C, sat M σ (a_exp (e_class e C)) ->
+                          C ∈ M ->
+                          sat M σ (a_intl e)
+
+  | sat_extl : forall M σ e C, sat M σ (a_exp (e_class e C)) ->
+                          ~ C ∈ M ->
+                          sat M σ (a_extl e)
 
   | sat_prt_from : forall M σ e e_orig α α_orig, eval M σ e (v_addr α) ->
                                             eval M σ e_orig (v_addr α_orig) ->
@@ -120,11 +170,64 @@ Module Assert.
                                                   is_protected_path M σ α_orig p) ->
                                             sat M σ (a_prt_frm e e_orig)
 
+  | sat_prt : forall M σ e, (forall α, loc_relevant α σ ->
+                             sat M σ (a_prt_frm e (e_val (v_addr α)))) ->
+                       sat M σ (a_prt e)
+
 
   with  nsat : module -> config -> asrt -> Prop :=
+
   | nsat_exp : forall M σ e, (forall v, eval M σ e v ->
                               v <> v_true) ->
-                        nsat M σ (a_exp e).
+                        nsat M σ (a_exp e)
+
+  | nsat_and1 : forall M σ A1 A2, nsat M σ A1 ->
+                             nsat M σ (A1 ∧ A2)
+
+  | nsat_and2 : forall M σ A1 A2, nsat M σ A2 ->
+                             nsat M σ (A1 ∧ A2)
+
+  | nsat_or : forall M σ A1 A2, nsat M σ A1 ->
+                           nsat M σ A2 ->
+                           nsat M σ (A1 ∨ A2)
+
+  | nsat_neg : forall M σ A, sat M σ A ->
+                        nsat M σ (¬ A)
+
+  | nsat_all : forall M σ x α A, glob_relevant α σ ->
+                            nsat M σ ([α /s 0] A) ->
+                            nsat M σ (a_all x A)
+
+  | nsat_ex : forall M σ x A, (forall α, glob_relevant α σ ->
+                                nsat M σ ([α /s 0] A)) ->
+                         nsat M σ (a_ex x A)
+
+  | nsat_intl : forall M σ e C, sat M σ (a_exp (e_class e C)) ->
+                           ~C ∈ M ->
+                           nsat M σ (a_intl e)
+
+  | nsat_extl : forall M σ e C, sat M σ (a_exp (e_class e C)) ->
+                           C ∈ M ->
+                           nsat M σ (a_extl e)
+
+  | nsat_prt_from1 : forall M σ e e_orig, (forall v α, eval M σ e v ->
+                                             v <> v_addr α) ->
+                                     nsat M σ (a_prt_frm e e_orig)
+
+  | nsat_prt_from2 : forall M σ e e_orig, (forall v_orig α, eval M σ e_orig v_orig ->
+                                                  v_orig <> v_addr α) ->
+                                     nsat M σ (a_prt_frm e e_orig)
+
+  | nsat_prt_from3 : forall M σ e e_orig v v_orig, eval M σ e v ->
+                                              eval M σ e_orig v_orig ->
+                                              v = v_orig ->
+                                              nsat M σ (a_prt_frm e e_orig)
+
+  | nsat_prt_from4 : forall M σ e e_orig α α_orig p, eval M σ e (v_addr α) ->
+                                                eval M σ e_orig (v_addr α_orig) ->
+                                                interpret_αp p σ α_orig = Some (v_addr α) ->
+                                                ~ is_protected_path M σ α_orig p ->
+                                                nsat M σ (a_prt_frm e e_orig).
 
 End Assert.
 
